abstract: manually import ARMv7a virtualisation extension spec
Gerwin imported this previously, but it required severe surgery to apply
that patch over the L4V_ARCH parametrisation of our specs (arch_split).

NOTE: This is the painfully hand-managed patch application. It will be rebased
again once it goes through Isabelle.

spec/abstract/ARM/Arch_Structs_A.thy
@@ -37,14 +37,61 @@ type_synonym vm_attributes = "vm_attribute set"
 section {* Architecture-specific capabilities *}
 
 text {*  The ARM kernel supports capabilities for ASID pools and an ASID controller capability,
-along with capabilities for page directories, page tables, and page mappings. *}
+along with capabilities for page tables, page mappings, System-MMU IO spaces, and 
+virtual CPU contexts for hyper calls. *}
+
+-- "up to three levels of translation, cf B3.3, pg 1318"
+datatype pt_level = PT_L1 | PT_L2 | PT_L3
+
+instantiation pt_level :: enum
+begin
+definition
+  enum_pt_level: "enum_class.enum \<equiv> [PT_L1,PT_L2,PT_L3]"
+definition 
+  "enum_class.enum_all (P::pt_level \<Rightarrow> bool) \<equiv> Ball UNIV P"
+definition
+  "enum_class.enum_ex (P::pt_level \<Rightarrow> bool) \<equiv> Bex UNIV P"
+instance
+  apply intro_classes
+  apply (safe, simp)
+  apply (case_tac x)
+  apply (auto simp: enum_pt_level enum_ex_pt_level_def enum_all_pt_level_def)
+  done
+end
+
+-- "all page tables take 4K, cf B3.3, pg 1318 (512 entries, 64 bit per entry)."
+definition
+  pt_bits :: "nat" where
+  "pt_bits \<equiv> 12"
+
+-- "cf B3.6, pg 1338"
+datatype vmpage_size =
+    ARM_1G_Block
+  | ARM_2M_Block
+  | ARM_4K_Page
+
+-- {* convert page size into bits, such that @{term "2^bits = sz"} *}
+definition
+  page_bits_for_size :: "vmpage_size \<Rightarrow> nat" where
+  "page_bits_for_size sz \<equiv> case sz of
+    ARM_1G_Block \<Rightarrow> 30
+  | ARM_2M_Block \<Rightarrow> 21
+  | ARM_4K_Page \<Rightarrow> 12"
+(* FIXME ARMHYP how is this related to pageBitsForSize? Equal modulo updating Haskell? *)
+
+-- "unique device identifiers, board/vendor specific"
+typedecl device_id
+
+text {* A page can either be mapped in a normal page table or an IO space  *}
+datatype mapping_root = MappedMem asid | MappedIO device_id
 
 datatype arch_cap =
    ASIDPoolCap obj_ref asid
  | ASIDControlCap
- | PageCap obj_ref cap_rights vmpage_size "(asid * vspace_ref) option"
- | PageTableCap obj_ref "(asid * vspace_ref) option"
- | PageDirectoryCap obj_ref "asid option"
+ | PageTableCap pt_level obj_ref "(mapping_root \<times> vspace_ref) option"
+ | PageCap obj_ref cap_rights vmpage_size "(mapping_root \<times> vspace_ref) option"
+ | IOSpaceCap "device_id option"
+ | VCPUCap obj_ref
 
 definition
   is_page_cap :: "arch_cap \<Rightarrow> bool" where
@@ -63,30 +110,66 @@ definition
 section {* Architecture-specific objects *}
 
 text {* This section gives the types and auxiliary definitions for the
-architecture-specific objects: a page directory entry (@{text "pde"})
-contains either an invalid entry, a page table reference, a section
-reference, or a super-section reference; a page table entry contains
+architecture-specific objects: a page table entry contains
 either an invalid entry, a large page, or a small page mapping;
+a virtual CPU object contains additional registers saved and restored
+for hyper calls;
 finally, an architecture-specific object is either an ASID pool, a
-page table, a page directory, or a data page used to model user
+page table, a virtual CPU, or a data page used to model user
 memory.
 *}
 
-datatype pde =
-   InvalidPDE
- | PageTablePDE obj_ref vm_attributes machine_word
- | SectionPDE obj_ref vm_attributes machine_word cap_rights
- | SuperSectionPDE obj_ref vm_attributes cap_rights
+text {*
+  Translation table format descriptors, or page table entries, cf B3.6.1, pg B3-1339.
 
+  @{text InvalidPTE} signifies unmapped or otherwise invalid entries, can be used at any level.
+  @{text TablePTE} points to a next-level tabel and can be used at levels 1 and 2.
+  Bits @{text "[39:12]"} of the PTE are bits @{text "[39:12]"} of the next-level page table.
+  We force bits @{text "[39:32]"} to 0. Page tables are 12-bit aligned, so bits @{text "[11:0]"}
+  of the output address are 0.
+  @{text Block_1G_PTE} points to a 1G block of memory from a 1st-level table. We model
+  stage 1 translations (32 bit input addresses), and force stage 2 translations to have
+  bits @{text "[39..32]"} set to 0. The two remaining bits are bits 31 and 30 of the 
+  output address (cf B3.6.1, pg 1340).
+  @{text Block_2M_PTE} points to a 2M block of memory from a 2nd-level table. Similarly
+  to 1G PTEs we force bits @{text "[39..32]"} set to 0. The remaining 11 bits @{text "[31:21]"}
+  of the PTE are bits @{text "[31:21]"} of the output address (cf B3.6.1, pg 1340).
+  @{text PagePTE} points to a 4K page of memory from a 3rd-level table. Similarly to table PTEs,
+  Bits @{text "[39:12]"} of the PTE are bits @{text "[39:12]"} of the output address.
+  Pages are 12-bit aligned, so bits @{text "[11:0]"} of the output address are 0.
+*}
 datatype pte =
    InvalidPTE
- | LargePagePTE obj_ref vm_attributes cap_rights
- | SmallPagePTE obj_ref vm_attributes cap_rights
+ | TablePTE "20 word" vm_attributes
+ | Block_1G_PTE "2 word" vm_attributes cap_rights
+ | Block_2M_PTE "11 word" vm_attributes cap_rights
+ | PagePTE "20 word" vm_attributes cap_rights
 
+definition
+  is_page :: "pte \<Rightarrow> bool"
+where
+  "is_page pte \<equiv> case pte of PagePTE _ _ _ \<Rightarrow> True | _  \<Rightarrow> False"
+
+definition
+  is_block :: "pte \<Rightarrow> bool"
+where
+  "is_block pte \<equiv> case pte of Block_1G_PTE _ _ _ \<Rightarrow> True | Block_2M_PTE _ _ _ \<Rightarrow> True | _ \<Rightarrow> False"
+
+typedecl hyper_reg -- "enumeration of additional hyper call registers"
+axiomatization where hyper_reg_enum_class: "OFCLASS(hyper_reg, enum_class)"
+instance hyper_reg :: enum by (rule hyper_reg_enum_class)
+
+type_synonym hyper_reg_context = "hyper_reg \<Rightarrow> 32 word"
+
+text {*
+  ASID pools translate 10 bits, VCPUs store a potential association to a TCB as well as 
+  an extended register context. Page tables have 512 entries (cf B3.6.5, pg 1348). For data pages,
+  we record their size.
+*}
 datatype arch_kernel_obj =
    ASIDPool "10 word \<rightharpoonup> obj_ref"
- | PageTable "word8 \<Rightarrow> pte"
- | PageDirectory "12 word \<Rightarrow> pde"
+ | VCPU "obj_ref option" hyper_reg_context
+ | PageTable "9 word \<Rightarrow> pte"
  | DataPage vmpage_size
 
 primrec
@@ -94,26 +177,29 @@ primrec
 where
   "arch_obj_size (ASIDPoolCap p as) = pageBits"
 | "arch_obj_size ASIDControlCap = 0"
-| "arch_obj_size (PageCap x rs sz as4) = pageBitsForSize sz"
-| "arch_obj_size (PageDirectoryCap x as2) = 14"
-| "arch_obj_size (PageTableCap x as3) = 10"
+| "arch_obj_size (PageCap _ _ sz _) = page_bits_for_size sz"
+| "arch_obj_size (PageTableCap _ _ _) = 12"
+| "arch_obj_size (VCPUCap _) = 11"
+| "arch_obj_size (IOSpaceCap _) = 0"
 
 primrec
   arch_kobj_size :: "arch_kernel_obj \<Rightarrow> nat"
 where
-  "arch_kobj_size (ASIDPool p) = pageBits"
-| "arch_kobj_size (PageTable pte) = 10"
-| "arch_kobj_size (PageDirectory pde) = 14"
-| "arch_kobj_size (DataPage sz) = pageBitsForSize sz"
+  "arch_kobj_size (ASIDPool _) = pageBits"
+| "arch_kobj_size (PageTable _) = pt_bits"
+| "arch_kobj_size (VCPU _ _) = 11"
+| "arch_kobj_size (DataPage sz) = page_bits_for_size sz"
+(* FIXME ARMHYP: vcpu_bits? *)
 
 primrec
   aobj_ref :: "arch_cap \<rightharpoonup> obj_ref"
 where
-  "aobj_ref (ASIDPoolCap p as) = Some p"
+  "aobj_ref (ASIDPoolCap p _) = Some p"
 | "aobj_ref ASIDControlCap = None"
-| "aobj_ref (PageCap x rs sz as4) = Some x"
-| "aobj_ref (PageDirectoryCap x as2) = Some x"
-| "aobj_ref (PageTableCap x as3) = Some x"
+| "aobj_ref (PageCap x _ _ _) = Some x"
+| "aobj_ref (PageTableCap _ x _) = Some x"
+| "aobj_ref (VCPUCap x) = Some x"
+| "aobj_ref (IOSpaceCap _) = None"
 
 primrec (nonexhaustive)
   acap_rights :: "arch_cap \<Rightarrow> cap_rights"
@@ -129,35 +215,32 @@ definition
 section {* Architecture-specific object types and default objects *}
 
 datatype
-  aobject_type = 
-    SmallPageObj
-  | LargePageObj
-  | SectionObj
-  | SuperSectionObj
-  | PageTableObj
-  | PageDirectoryObj
+  aobject_type =
+    ARM_4K_PageObj
+  | ARM_2M_BlockObj
+  | ARM_1G_BlockObj
+  | PageTableObj pt_level
+  | VCPUObj
   | ASIDPoolObj
 
 definition
   arch_default_cap :: "aobject_type \<Rightarrow> obj_ref \<Rightarrow> nat \<Rightarrow> arch_cap" where
  "arch_default_cap tp r n \<equiv> case tp of
-  SmallPageObj \<Rightarrow> PageCap r vm_read_write ARMSmallPage None
-  | LargePageObj \<Rightarrow> PageCap r vm_read_write ARMLargePage None
-  | SectionObj \<Rightarrow> PageCap r vm_read_write ARMSection None
-  | SuperSectionObj \<Rightarrow> PageCap r vm_read_write ARMSuperSection None
-  | PageTableObj \<Rightarrow> PageTableCap r None
-  | PageDirectoryObj \<Rightarrow> PageDirectoryCap r None
+    ARM_4K_PageObj \<Rightarrow> PageCap r vm_read_write ARM_4K_Page None
+  | ARM_2M_BlockObj \<Rightarrow> PageCap r vm_read_write ARM_2M_Block None
+  | ARM_1G_BlockObj \<Rightarrow> PageCap r vm_read_write ARM_1G_Block None
+  | PageTableObj l \<Rightarrow> PageTableCap l r None
+  | VCPUObj \<Rightarrow> VCPUCap r
   | ASIDPoolObj \<Rightarrow> ASIDPoolCap r 0" (* unused *)
 
 definition
   default_arch_object :: "aobject_type \<Rightarrow> nat \<Rightarrow> arch_kernel_obj" where
  "default_arch_object tp n \<equiv> case tp of
-    SmallPageObj \<Rightarrow> DataPage ARMSmallPage 
-  | LargePageObj \<Rightarrow> DataPage ARMLargePage
-  | SectionObj \<Rightarrow> DataPage ARMSection
-  | SuperSectionObj \<Rightarrow> DataPage ARMSuperSection
-  | PageTableObj \<Rightarrow> PageTable (\<lambda>x. InvalidPTE)
-  | PageDirectoryObj \<Rightarrow> PageDirectory (\<lambda>x. InvalidPDE)
+    ARM_4K_PageObj \<Rightarrow> DataPage ARM_4K_Page
+  | ARM_2M_BlockObj \<Rightarrow> DataPage ARM_2M_Block
+  | ARM_1G_BlockObj \<Rightarrow> DataPage ARM_1G_Block
+  | PageTableObj _ \<Rightarrow> PageTable (\<lambda>x. InvalidPTE)
+  | VCPUObj \<Rightarrow> VCPU None (\<lambda>x. 0)
   | ASIDPoolObj \<Rightarrow> ASIDPool (\<lambda>_. None)"
 
 type_synonym hw_asid = word8
@@ -188,16 +271,9 @@ record arch_state =
   arm_hwasid_table  :: "hw_asid \<rightharpoonup> asid"
   arm_next_asid     :: hw_asid
   arm_asid_map      :: "asid \<rightharpoonup> (hw_asid \<times> obj_ref)"
-  arm_global_pd     :: obj_ref
-  arm_global_pts    :: "obj_ref list"
+  arm_global_l1_pt  :: obj_ref
+  arm_global_l2_pts :: "obj_ref list"
   arm_kernel_vspace :: arm_vspace_region_uses
-
-definition
-  pd_bits :: "nat" where
-  "pd_bits \<equiv> pageBits + 2"
-
-definition
-  pt_bits :: "nat" where
-  "pt_bits \<equiv> pageBits - 2"
+  arm_io_space      :: "device_id \<rightharpoonup> obj_ref"
 
 end
