spec/abstract/ARM/ArchEncoding_A.thy
@@ -1,0 +1,64 @@
+header "Encoding ARM VSpace concepts"
+
+theory ArchEncoding_A imports
+  ArchVSpace_A
+begin
+
+text {* 
+  Convert a set of rights into binary form.
+  @{text "AP[2:1]"} permission model, cf. B3.7.1, pg 1357.
+  For stage 1 translations:
+  0 means kernel-only (PL1) access (read/write),
+  1 means read/write at any privilege level,
+  2 means read-only for user-level (PL0), read-write for kernel (PL1).
+*}
+definition
+  word_from_vm_rights :: "vm_rights \<Rightarrow> word32" where  
+  "word_from_vm_rights R \<equiv> 
+  if vm_read_write \<subseteq> R then 1
+  else if vm_read_only \<subseteq> R then 2
+  else 0"
+
+
+text {* The vm rights of a PTE. Empty if not applicable. *}
+fun
+  vm_rights_of :: "pte \<Rightarrow> cap_rights"
+where
+  "vm_rights_of (Block_1G_PTE _ _ rights) = rights" |
+  "vm_rights_of (Block_2M_PTE _ _ rights) = rights" |
+  "vm_rights_of (PagePTE _ _ rights) = rights" |
+  "vm_rights_of _ = {}"
+
+text {* The vm attributes of a PTE. Empty if not applicable. *}
+fun
+  vm_attribs_of :: "pte \<Rightarrow> vm_attributes"
+where
+  "vm_attribs_of (Block_1G_PTE _ attrs _) = attrs" |
+  "vm_attribs_of (Block_2M_PTE _ attrs _) = attrs" |
+  "vm_attribs_of (PagePTE _ attrs _) = attrs" |
+  "vm_attribs_of _ = {}"
+
+text {*
+  Encoding of VM attributes as in stage 1 block and page descriptors (cf B3.6.2, pg 1342).
+  We only allow users to specify the Cacheable attribute, which translates to 
+  Write-Back, Write-Allocate (cf B3.8.2, pg 1367).
+  This assumes TRE == 0 Remap disabled (cf B3.8.1, pg 1366).
+*}
+definition
+  word_from_vmattr :: "vm_attributes \<Rightarrow> machine_word"
+where
+  "word_from_vmattr attr \<equiv> if PageCacheable \<in> attr then 0b110 else 0"
+
+text {* Encode a page table entry into the equivalent entry that the page
+table walker implemented in ARM hardware would parse, cf B3.6.1. *}
+definition
+  word_from_pte :: "pte \<Rightarrow> machine_word" where
+  "word_from_pte pte \<equiv> 
+    (if pte = InvalidPTE then 0 
+     else if is_block pte then 1
+     else 0b11) ||
+    addr_from_pte pte ||
+    (word_from_vmattr (vm_attribs_of pte) << 2) ||
+    (word_from_vm_rights (vm_rights_of pte) << 6)"
+
+end
