spec/abstract/ARM/ArchRetype_A.thy
@@ -26,7 +26,7 @@ definition
   reserve_region :: "obj_ref \<Rightarrow> nat \<Rightarrow> bool \<Rightarrow> (unit,'z::state_ext) s_monad" where
   "reserve_region ptr byteLength is_kernel \<equiv> return ()"
 
-text {* Create 4096-byte frame objects that can be mapped into memory. These must be
+text {* Create 4k frame objects that can be mapped into memory. These must be
 cleared to prevent past contents being revealed. *}
 
 definition
@@ -35,7 +35,7 @@ definition
   do
     byteLength \<leftarrow> return $ numObjects * 2 ^ sz;
     reserve_region ptr byteLength True;
-    rst \<leftarrow>  return (map (\<lambda> n. (ptr + (n << sz))) [0  .e.  (of_nat numObjects) - 1]);
+    rst \<leftarrow> return (map (\<lambda> n. (ptr + (n << sz))) [0  .e.  (of_nat numObjects) - 1]);
     do_machine_op $ mapM_x (\<lambda>x. clearMemory x (2 ^ sz)) rst
  od"
 
@@ -45,18 +45,16 @@ definition
   init_arch_objects :: "apiobject_type \<Rightarrow> obj_ref \<Rightarrow> nat \<Rightarrow> nat \<Rightarrow> obj_ref list \<Rightarrow> (unit,'z::state_ext) s_monad"
 where
   "init_arch_objects new_type ptr num_objects obj_sz refs \<equiv> case new_type of
-    ArchObject SmallPageObj \<Rightarrow> create_word_objects ptr num_objects 12
-  | ArchObject LargePageObj \<Rightarrow> create_word_objects ptr num_objects 16
-  | ArchObject SectionObj \<Rightarrow> create_word_objects ptr num_objects 20
-  | ArchObject SuperSectionObj \<Rightarrow> create_word_objects ptr num_objects 24
-  | ArchObject PageTableObj \<Rightarrow>
-      do_machine_op $ mapM_x (\<lambda>x. cleanCacheRange_PoU x (x + ((1::word32) << pt_bits) - 1)
-                                                      (addrFromPPtr x)) refs
-  | ArchObject PageDirectoryObj \<Rightarrow> do
+    ArchObject ARM_4K_PageObj \<Rightarrow> create_word_objects ptr num_objects 12
+  | ArchObject ARM_2M_BlockObj \<Rightarrow> create_word_objects ptr num_objects 21
+  | ArchObject ARM_1G_BlockObj \<Rightarrow> create_word_objects ptr num_objects 30
+  | ArchObject (PageTableObj PT_L1) \<Rightarrow> do
       mapM_x copy_global_mappings refs;
-      do_machine_op $ mapM_x (\<lambda>x. cleanCacheRange_PoU x (x + ((1::word32) << pd_bits) - 1)
-                                                      (addrFromPPtr x)) refs
+      do_machine_op $ mapM_x (\<lambda>x. cleanCacheRange_PoU x (x + ((1::word32) << pt_bits) - 1) (addrFromPPtr x)) refs
+  | ArchObject (PageTableObj _) \<Rightarrow>
+      do_machine_op $ mapM_x (\<lambda>x. cleanCacheRange_PoU x (x + ((1::word32) << pt_bits) - 1) (addrFromPPtr x)) refs
     od
   | _ \<Rightarrow> return ()"
+(* FIXME ARMHYP: the two PageTableObj init cases can be folded by using an if l = PT_L1 *)
 
 end
