spec/abstract/ARM/ArchVSpaceAcc_A.thy
@@ -54,45 +54,25 @@ definition
   od"
 
 definition
-  get_pd :: "obj_ref \<Rightarrow> (12 word \<Rightarrow> pde,'z::state_ext) s_monad" where
-  "get_pd ptr \<equiv> do
+  get_vcpu :: "obj_ref \<Rightarrow> (obj_ref option \<times> hyper_reg_context,'z::state_ext) s_monad" where
+  "get_vcpu ptr \<equiv> do
      kobj \<leftarrow> get_object ptr;
-     (case kobj of ArchObj (PageDirectory pd) \<Rightarrow> return pd
+     (case kobj of ArchObj (VCPU t r) \<Rightarrow> return (t,r)
                  | _ \<Rightarrow> fail)
    od"
 
 definition
-  set_pd :: "obj_ref \<Rightarrow> (12 word \<Rightarrow> pde) \<Rightarrow> (unit,'z::state_ext) s_monad" where
-  "set_pd ptr pd \<equiv> do
+  set_vcpu :: "obj_ref \<Rightarrow> (obj_ref option \<times> hyper_reg_context) \<Rightarrow> (unit,'z::state_ext) s_monad"
+where
+  "set_vcpu ptr vcpu \<equiv> do
+     (t,r) \<leftarrow> return vcpu;
      kobj \<leftarrow> get_object ptr;
-     assert (case kobj of ArchObj (PageDirectory pd) \<Rightarrow> True | _ \<Rightarrow> False);
-     set_object ptr (ArchObj (PageDirectory pd)) 
-   od"
-
-text {* The following function takes a pointer to a PDE in kernel memory
-  and returns the actual PDE. *}
-definition
-  get_pde :: "obj_ref \<Rightarrow> (pde,'z::state_ext) s_monad" where
-  "get_pde ptr \<equiv> do
-     base \<leftarrow> return (ptr && ~~mask pd_bits);
-     offset \<leftarrow> return ((ptr && mask pd_bits) >> 2);
-     pd \<leftarrow> get_pd base;
-     return $ pd (ucast offset)
+     assert (case kobj of ArchObj (VCPU _ _) \<Rightarrow> True | _ \<Rightarrow> False);
+     set_object ptr (ArchObj (VCPU t r))
    od"
 
 definition
-  store_pde :: "obj_ref \<Rightarrow> pde \<Rightarrow> (unit,'z::state_ext) s_monad" where
-  "store_pde p pde \<equiv> do
-    base \<leftarrow> return (p && ~~mask pd_bits);
-    offset \<leftarrow> return ((p && mask pd_bits) >> 2);
-    pd \<leftarrow> get_pd base;
-    pd' \<leftarrow> return $ pd (ucast offset := pde);
-    set_pd base pd'
-  od"
-
-
-definition
-  get_pt :: "obj_ref \<Rightarrow> (word8 \<Rightarrow> pte,'z::state_ext) s_monad" where
+  get_pt :: "obj_ref \<Rightarrow> (9 word \<Rightarrow> pte,'z::state_ext) s_monad" where
   "get_pt ptr \<equiv> do
      kobj \<leftarrow> get_object ptr;
      (case kobj of ArchObj (PageTable pt) \<Rightarrow> return pt
@@ -100,7 +80,7 @@ definition
    od"
 
 definition
-  set_pt :: "obj_ref \<Rightarrow> (word8 \<Rightarrow> pte) \<Rightarrow> (unit,'z::state_ext) s_monad" where
+  set_pt :: "obj_ref \<Rightarrow> (9 word \<Rightarrow> pte) \<Rightarrow> (unit,'z::state_ext) s_monad" where
   "set_pt ptr pt \<equiv> do
      kobj \<leftarrow> get_object ptr;
      assert (case kobj of ArchObj (PageTable _) \<Rightarrow> True | _ \<Rightarrow> False);
@@ -113,7 +93,7 @@ definition
   get_pte :: "obj_ref \<Rightarrow> (pte,'z::state_ext) s_monad" where
   "get_pte ptr \<equiv> do
      base \<leftarrow> return (ptr && ~~mask pt_bits);
-     offset \<leftarrow> return ((ptr && mask pt_bits) >> 2);
+     offset \<leftarrow> return (ptr && mask pt_bits >> 3);
      pt \<leftarrow> get_pt base;
      return $ pt (ucast offset)
    od"
@@ -122,7 +102,7 @@ definition
   store_pte :: "obj_ref \<Rightarrow> pte \<Rightarrow> (unit,'z::state_ext) s_monad" where
   "store_pte p pte \<equiv> do
     base \<leftarrow> return (p && ~~mask pt_bits);
-    offset \<leftarrow> return ((p && mask pt_bits) >> 2);
+    offset \<leftarrow> return (p && mask pt_bits >> 2);
     pt \<leftarrow> get_pt base;
     pt' \<leftarrow> return $ pt (ucast offset := pte);
     set_pt base pt'
@@ -136,45 +116,81 @@ text {* The kernel window is mapped into every virtual address space from the
 create the kernel window into a new page directory object. *}
 definition
 copy_global_mappings :: "obj_ref \<Rightarrow> (unit,'z::state_ext) s_monad" where
-"copy_global_mappings new_pd \<equiv> do
-    global_pd \<leftarrow> gets (arm_global_pd \<circ> arch_state);
-    pde_bits \<leftarrow> return 2;
-    pd_size \<leftarrow> return (1 << (pd_bits - pde_bits));
+"copy_global_mappings new_pt \<equiv> do
+    global_pt \<leftarrow> gets (arm_global_l1_pt \<circ> arch_state);
+    pte_bits \<leftarrow> return 3;
+    pd_size \<leftarrow> return (1 << (pt_bits - pte_bits));
     mapM_x (\<lambda>index. do
-        offset \<leftarrow> return (index << pde_bits);
-        pde \<leftarrow> get_pde (global_pd + offset);
-        store_pde (new_pd + offset) pde
+        offset \<leftarrow> return (index << pte_bits);
+        pde \<leftarrow> get_pte (global_pt + offset);
+        store_pte (new_pt + offset) pde
     od) [kernel_base >> 20  .e.  pd_size - 1] 
 od"
 
-text {* Walk the page directories and tables in software. *}
+text {* Walk the page tables in software. *}
 
-text {* The following function takes a page-directory reference as well as
-  a virtual address and then computes a pointer to the PDE in kernel memory *}
 definition
-lookup_pd_slot :: "word32 \<Rightarrow> vspace_ref \<Rightarrow> word32" where
-"lookup_pd_slot pd vptr \<equiv>
-    let pd_index = vptr >> 20
-    in pd + (pd_index << 2)"
+  bit_slice :: "'a::len word \<Rightarrow> nat \<Rightarrow> nat \<Rightarrow> 'a word" ("_[_:_]" [70,0,0] 71)
+where
+  "w[n:m] = w && mask (n + 1) && ~~ mask m"
 
-text {* The following function takes a page-directory reference as well as
-  a virtual address and then computes a pointer to the PTE in kernel memory.
-  Note that the function fails if the virtual address is mapped on a section or
-  super section. *}
+definition level_bits :: "pt_level \<Rightarrow> nat" where
+  "level_bits level \<equiv> case level of
+    PT_L1 \<Rightarrow> 30
+  | PT_L2 \<Rightarrow> 21
+  | PT_L3 \<Rightarrow> pt_bits"
+
+definition pt_index_of :: "pt_level \<Rightarrow> vspace_ref \<Rightarrow> 32 word" where
+  "pt_index_of l va \<equiv> let m = level_bits l in
+  (case l of
+    PT_L1 \<Rightarrow> va[31:m]
+  | PT_L2 \<Rightarrow> va[29:m]
+  | PT_L3 \<Rightarrow> va[30:m]) >> m"
+
+text {*
+  Return reference to the PTE addressed by @{text vspace_ref} in
+  a page table located at @{term pt}, assuming the table is at level @{term l}
+*}
 definition
-lookup_pt_slot :: "word32 \<Rightarrow> vspace_ref \<Rightarrow> (word32,'z::state_ext) lf_monad" where
-"lookup_pt_slot pd vptr \<equiv> doE
-    pd_slot \<leftarrow> returnOk (lookup_pd_slot pd vptr); 
-    pde \<leftarrow> liftE $ get_pde pd_slot;
-    (case pde of
-          PageTablePDE ptab _ _ \<Rightarrow>   (doE
-            pt \<leftarrow> returnOk (ptrFromPAddr ptab);
-            pt_index \<leftarrow> returnOk ((vptr >> 12) && 0xff);
-            pt_slot \<leftarrow> returnOk (pt + (pt_index << 2));
-            returnOk pt_slot
-          odE)
-        | _ \<Rightarrow> throwError $ MissingCapability 20)
-odE"
+  pte_slot :: "pt_level \<Rightarrow> obj_ref \<Rightarrow> vspace_ref \<Rightarrow> obj_ref"
+where
+  "pte_slot l pt va \<equiv> pt || (pt_index_of l va << 3)"
+
+text {*
+  Look up the (kernel-memory) address of the next-level page table.
+  @{text pt_ref} is assumed to be a table at level @{text l}.
+  Fails if the PTE is Invalid, Page, or Block.
+*}
+definition
+  lookup_pt :: "pt_level \<Rightarrow> obj_ref \<Rightarrow> vspace_ref \<Rightarrow> (obj_ref,'z::state_ext) lf_monad" where
+  "lookup_pt l pt_ref vptr = doE
+    pt_slot \<leftarrow> returnOk (pte_slot l pt_ref vptr);
+    pte \<leftarrow> liftE $ get_pte pt_slot;
+    (case pte of
+      TablePTE ptab _ \<Rightarrow> returnOk $ ptrFromPAddr (ucast ptab << pt_bits)
+    | _ \<Rightarrow> throwError $ MissingCapability 20)
+  odE"
+
+text {* Look up the (kernel-memory) address of the PTE in the
+  page table specified by @{text vptr}, from page table root
+  @{text pt_ref}, translating up to the specified level.
+  Fails if any of the translation steps are via TablePTEs. *}
+fun
+  lookup_pt_slot :: "pt_level \<Rightarrow> obj_ref \<Rightarrow> vspace_ref \<Rightarrow> (obj_ref,'z::state_ext) lf_monad"
+where
+  "lookup_pt_slot PT_L1 pt vptr =
+    returnOk (pte_slot PT_L1 pt vptr)"
+|
+  "lookup_pt_slot PT_L2 pt vptr = doE
+    pt2 \<leftarrow> lookup_pt PT_L1 pt vptr;
+    returnOk $ pte_slot PT_L2 pt2 vptr
+  odE"
+|
+  "lookup_pt_slot PT_L3 pt vptr = doE
+    pt2 \<leftarrow> lookup_pt PT_L1 pt vptr;
+    pt3 \<leftarrow> lookup_pt PT_L2 pt2 vptr;
+    returnOk $ pte_slot PT_L3 pt3 vptr
+  odE"
 
 
 text {* A non-failing version of @{const lookup_pt_slot} when the pd is already known *}
