spec/abstract/ARM/ArchVSpace_A.thy
@@ -18,103 +18,66 @@ theory ArchVSpace_A
 imports "../Retype_A"
 begin
 
-text {* Save the set of entries that would be inserted into a page table or
-page directory to map various different sizes of frame at a given virtual
-address. *}
-fun create_mapping_entries ::
+text {* Save the set of entries that would be inserted into a page table
+ to map various different sizes of frame at a given virtual address. *}
+fun create_mapping_entry ::
   "paddr \<Rightarrow> vspace_ref \<Rightarrow> vmpage_size \<Rightarrow> vm_rights \<Rightarrow> vm_attributes \<Rightarrow> word32 \<Rightarrow>
-  ((pte * word32 list) + (pde * word32 list),'z::state_ext) se_monad"
+  (pte \<times> obj_ref,'z::state_ext) se_monad"
 where
-  "create_mapping_entries base vptr ARMSmallPage vm_rights attrib pd =
+  "create_mapping_entry base vptr ARM_4K_Page vm_rights attrib pt =
   doE
-    p \<leftarrow> lookup_error_on_failure False $ lookup_pt_slot pd vptr;
-    returnOk $ Inl (SmallPagePTE base (attrib - {Global, ParityEnabled})
-                                 vm_rights, [p])
+    pte_ref \<leftarrow> lookup_error_on_failure False $ lookup_pt_slot PT_L3 pt vptr;
+    returnOk (PagePTE (ucast (base >> page_bits_for_size ARM_4K_Page))
+                      (attrib - {Global, ParityEnabled}) vm_rights, pte_ref)
+  odE"
+|
+  "create_mapping_entry base vptr ARM_2M_Block vm_rights attrib pt =
+  doE
+    pte_ref \<leftarrow> lookup_error_on_failure False $ lookup_pt_slot PT_L2 pt vptr;
+    returnOk (Block_2M_PTE (ucast (base >> page_bits_for_size ARM_2M_Block))
+                           (attrib - {Global, ParityEnabled}) vm_rights, pte_ref)
+  odE"
+|
+  "create_mapping_entry base vptr ARM_1G_Block vm_rights attrib pt =
+  doE
+    pte_ref \<leftarrow> lookup_error_on_failure False $ lookup_pt_slot PT_L1 pt vptr;
+    returnOk (Block_2M_PTE (ucast (base >> page_bits_for_size ARM_1G_Block))
+                           (attrib - {Global, ParityEnabled}) vm_rights, pte_ref)
   odE"
 
-| "create_mapping_entries base vptr ARMLargePage vm_rights attrib pd =
-  doE
-    p \<leftarrow> lookup_error_on_failure False $ lookup_pt_slot pd vptr;
-    returnOk $ Inl (LargePagePTE base (attrib - {Global, ParityEnabled})
-                                 vm_rights, [p, p + 4  .e.  p + 60])
-  odE"
 
-| "create_mapping_entries base vptr ARMSection vm_rights attrib pd =
-  doE
-    p \<leftarrow> returnOk (lookup_pd_slot pd vptr);
-    returnOk $ Inr (SectionPDE base (attrib - {Global}) 0 vm_rights, [p])
-  odE"
-
-| "create_mapping_entries base vptr ARMSuperSection vm_rights attrib pd =
-  doE
-    p \<leftarrow> returnOk (lookup_pd_slot pd vptr);
-    returnOk $ Inr (SuperSectionPDE base (attrib - {Global}) vm_rights, [p, p + 4  .e.  p + 60])
-  odE"
-
-definition get_master_pde :: "word32 \<Rightarrow> (Arch_Structs_A.pde,'z::state_ext)s_monad"
-  where "get_master_pde ptr \<equiv> do
-    pde \<leftarrow> (get_pde (ptr && ~~ mask 6));
-    (case pde of Arch_Structs_A.pde.SuperSectionPDE _ _ _ \<Rightarrow> return pde
-    | _ \<Rightarrow> get_pde ptr)
-  od"
-
-definition get_master_pte :: "word32 \<Rightarrow> (Arch_Structs_A.pte, 'z::state_ext)s_monad"
-  where "get_master_pte ptr \<equiv> do
-    pte \<leftarrow> (get_pte (ptr && ~~ mask 6));
-    (case pte of Arch_Structs_A.pte.LargePagePTE _ _ _ \<Rightarrow> return pte
-    | _ \<Rightarrow> get_pte ptr)
-  od"
-
-text {* Placing an entry which maps a frame within the set of entries that map a
-larger frame is unsafe. This function checks that given entries replace either
-invalid entries or entries of the same granularity. *}
+text {* This function checks that given entries replace either
+invalid entries or existing frames of the same size, but not page tables. *}
 fun ensure_safe_mapping ::
-  "(pte * word32 list) + (pde * word32 list) \<Rightarrow> (unit,'z::state_ext) se_monad"
+  "pte \<times> word32 \<Rightarrow> (unit,'z::state_ext) se_monad"
 where
-"ensure_safe_mapping (Inl (InvalidPTE, _)) = returnOk ()"
+"ensure_safe_mapping (InvalidPTE, _) = returnOk ()"
 |
-"ensure_safe_mapping (Inl (SmallPagePTE _ _ _, pt_slots)) =
-    mapME_x (\<lambda>slot. (doE
-        pte \<leftarrow> liftE $ get_master_pte slot;
-        (case pte of
-              InvalidPTE \<Rightarrow> returnOk ()
-            | SmallPagePTE _ _ _ \<Rightarrow> returnOk ()
-            | _ \<Rightarrow> throwError DeleteFirst)
-    odE)) pt_slots"
+"ensure_safe_mapping (PagePTE _ _ _, slot) = doE
+  pte \<leftarrow> liftE $ get_pte slot;
+  (case pte of
+    InvalidPTE \<Rightarrow> returnOk ()
+  | PagePTE _ _ _ \<Rightarrow> returnOk ()
+  | _ \<Rightarrow> throwError DeleteFirst)
+odE"
 |
-"ensure_safe_mapping (Inl (LargePagePTE _ _ _, pt_slots)) =
-    mapME_x (\<lambda> slot. (doE
-        pte \<leftarrow> liftE $ get_master_pte slot;
-        (case pte of
-              InvalidPTE \<Rightarrow> returnOk ()
-            | LargePagePTE _ _ _ \<Rightarrow> returnOk ()
-            | _ \<Rightarrow> throwError DeleteFirst
-            )
-    odE)) pt_slots"
+"ensure_safe_mapping (Block_2M_PTE _ _ _, slot) = doE
+  pte \<leftarrow> liftE $ get_pte slot;
+  (case pte of
+    InvalidPTE \<Rightarrow> returnOk ()
+  | Block_2M_PTE _ _ _ \<Rightarrow> returnOk ()
+  | _ \<Rightarrow> throwError DeleteFirst)
+odE"
 |
-"ensure_safe_mapping (Inr (InvalidPDE, _)) = returnOk ()"
+"ensure_safe_mapping (Block_1G_PTE _ _ _, slot) = doE
+  pte \<leftarrow> liftE $ get_pte slot;
+  (case pte of
+    InvalidPTE \<Rightarrow> returnOk ()
+  | Block_1G_PTE _ _ _ \<Rightarrow> returnOk ()
+  | _ \<Rightarrow> throwError DeleteFirst)
+odE"
 |
-"ensure_safe_mapping (Inr (PageTablePDE _ _ _, _)) = fail"
-|
-"ensure_safe_mapping (Inr (SectionPDE _ _ _ _, pd_slots)) =
-    mapME_x (\<lambda> slot. (doE
-        pde \<leftarrow> liftE $ get_master_pde slot;
-        (case pde of
-              InvalidPDE \<Rightarrow> returnOk ()
-            | SectionPDE _ _ _ _ \<Rightarrow> returnOk ()
-            | _ \<Rightarrow> throwError DeleteFirst
-            )
-    odE)) pd_slots"
-|
-"ensure_safe_mapping (Inr (SuperSectionPDE _ _ _, pd_slots)) =
-    mapME_x (\<lambda> slot. (doE
-        pde \<leftarrow> liftE $ get_master_pde slot;
-        (case pde of
-              InvalidPDE \<Rightarrow> returnOk ()
-            | SuperSectionPDE _ _ _ \<Rightarrow> returnOk ()
-            | _ \<Rightarrow> throwError DeleteFirst
-            )
-    odE)) pd_slots"
+"ensure_safe_mapping (TablePTE _ _, slot) = fail"
 
 text {* Look up a thread's IPC buffer and check that the thread has the right
 authority to read or (in the receiver case) write to it. *}
@@ -127,23 +90,23 @@ lookup_ipc_buffer :: "bool \<Rightarrow> word32 \<Rightarrow> (word32 option,'z:
     (case buffer_cap of
       ArchObjectCap (PageCap p R vms _) \<Rightarrow>
         if vm_read_write \<subseteq> R \<or> vm_read_only \<subseteq> R \<and> \<not>is_receiver
-        then return $ Some $ p + (buffer_ptr && mask (pageBitsForSize vms))
+        then return $ Some $ p + (buffer_ptr && mask (page_bits_for_size vms))
         else return None
     | _ \<Rightarrow> return None)
 od"
 
 text {* Locate the page directory associated with a given virtual ASID. *}
 definition
-find_pd_for_asid :: "asid \<Rightarrow> (word32,'z::state_ext) lf_monad" where
-"find_pd_for_asid asid \<equiv> doE
+find_pt_for_asid :: "asid \<Rightarrow> (word32,'z::state_ext) lf_monad" where
+"find_pt_for_asid asid \<equiv> doE
     assertE (asid > 0);
     asid_table \<leftarrow> liftE $ gets (arm_asid_table \<circ> arch_state);
     pool_ptr \<leftarrow> returnOk (asid_table (asid_high_bits_of asid));
     pool \<leftarrow> (case pool_ptr of
                Some ptr \<Rightarrow> liftE $ get_asid_pool ptr
              | None \<Rightarrow> throwError InvalidRoot);
-    pd \<leftarrow> returnOk (pool (ucast asid));
-    (case pd of
+    pt \<leftarrow> returnOk (pool (ucast asid));
+    (case pt of
           Some ptr \<Rightarrow> returnOk ptr
         | None \<Rightarrow> throwError InvalidRoot)
 odE"
@@ -151,12 +114,32 @@ odE"
 text {* Locate the page directory and check that this process succeeds and
 returns a pointer to a real page directory. *}
 definition
-find_pd_for_asid_assert :: "asid \<Rightarrow> (word32,'z::state_ext) s_monad" where
-"find_pd_for_asid_assert asid \<equiv> do
-   pd \<leftarrow> find_pd_for_asid asid <catch> K fail;
-   get_pde pd;
-   return pd
+find_pt_for_asid_assert :: "asid \<Rightarrow> (word32,'z::state_ext) s_monad" where
+"find_pt_for_asid_assert asid \<equiv> do
+   pt \<leftarrow> find_pt_for_asid asid <catch> K fail;
+   get_pte pt;
+   return pt
  od"
+
+definition
+  get_io_pt :: "device_id \<Rightarrow> (obj_ref option,'z::state_ext) s_monad"
+where
+  "get_io_pt dev \<equiv> gets (\<lambda>s. (arm_io_space \<circ> arch_state) s dev)"
+
+text {* Get the root page table of a specific device *}
+definition
+find_pt_for_device :: "device_id \<Rightarrow> (obj_ref,'z::state_ext) lf_monad" where
+"find_pt_for_device dev = doE
+   opt_pt \<leftarrow> liftE $ get_io_pt dev;
+   throw_opt InvalidRoot opt_pt
+odE"
+
+text {* Get the root page table of a specific mapping root (asid or device id) *}
+definition
+find_root_pt :: "mapping_root \<Rightarrow> (obj_ref,'z::state_ext) lf_monad" where
+"find_root_pt m \<equiv> case m of
+    MappedMem asid \<Rightarrow> find_pt_for_asid asid
+  | MappedIO dev \<Rightarrow> find_pt_for_device dev"
 
 text {* Format a VM fault message to be passed to a thread's supervisor after
 it encounters a page fault. *}
@@ -188,9 +171,9 @@ text {* Associate a hardware ASID with a virtual ASID. *}
 definition
 store_hw_asid :: "asid \<Rightarrow> hardware_asid \<Rightarrow> (unit,'z::state_ext) s_monad" where
 "store_hw_asid asid hw_asid \<equiv> do
-    pd \<leftarrow> find_pd_for_asid_assert asid;
+    pt \<leftarrow> find_pt_for_asid_assert asid;
     asid_map \<leftarrow> gets (arm_asid_map \<circ> arch_state);
-    asid_map' \<leftarrow> return (asid_map (asid \<mapsto> (hw_asid, pd)));
+    asid_map' \<leftarrow> return (asid_map (asid \<mapsto> (hw_asid, pt)));
     modify (\<lambda>s. s \<lparr> arch_state := (arch_state s) \<lparr> arm_asid_map := asid_map' \<rparr>\<rparr>);
     hw_asid_map \<leftarrow> gets (arm_hwasid_table \<circ> arch_state);
     hw_asid_map' \<leftarrow> return (hw_asid_map (hw_asid \<mapsto> asid));
@@ -293,9 +276,9 @@ abbreviation
 definition
   arm_context_switch :: "word32 \<Rightarrow> asid \<Rightarrow> (unit, 'z::state_ext) s_monad"
 where
-  "arm_context_switch pd asid \<equiv> do
+  "arm_context_switch pt asid \<equiv> do
       hwasid \<leftarrow> get_hw_asid asid;
-      do_machine_op $ arm_context_switch_hwasid pd hwasid
+      do_machine_op $ arm_context_switch_hwasid pt hwasid
     od"
 
 text {* Switch into the address space of a given thread or the global address
@@ -306,15 +289,15 @@ definition
     thread_root_slot \<leftarrow> return (tcb, tcb_cnode_index 1);
     thread_root \<leftarrow> get_cap thread_root_slot;
     (case thread_root of
-       ArchObjectCap (PageDirectoryCap pd (Some asid)) \<Rightarrow> doE
-           pd' \<leftarrow> find_pd_for_asid asid;
-           whenE (pd \<noteq> pd') $ throwError InvalidRoot;
-           liftE $ arm_context_switch pd asid
+       ArchObjectCap (PageTableCap PT_L1 pt (Some (MappedMem asid, _))) \<Rightarrow> doE
+           pt' \<leftarrow> find_pt_for_asid asid;
+           whenE (pt \<noteq> pt') $ throwError InvalidRoot;
+           liftE $ arm_context_switch pt asid
        odE
      | _ \<Rightarrow> throwError InvalidRoot) <catch>
     (\<lambda>_. do
-       global_pd \<leftarrow> gets (arm_global_pd \<circ> arch_state);
-       do_machine_op $ setCurrentPD $ addrFromPPtr global_pd
+       global_pt \<leftarrow> gets (arm_global_l1_pt \<circ> arch_state);
+       do_machine_op $ setCurrentPD $ addrFromPPtr global_pt
     od)
 od"
 
@@ -338,17 +321,16 @@ delete_asid_pool :: "asid \<Rightarrow> word32 \<Rightarrow> (unit,'z::state_ext
   od
 od"
 
-text {* When deleting a page directory from an ASID pool we must deactivate
-it. *}
+text {* When deleting a page table from an ASID pool we must deactivate it. *}
 definition
 delete_asid :: "asid \<Rightarrow> word32 \<Rightarrow> (unit,'z::state_ext) s_monad" where
-"delete_asid asid pd \<equiv> do
+"delete_asid asid pt \<equiv> do
   asid_table \<leftarrow> gets (arm_asid_table \<circ> arch_state);
   (case asid_table (asid_high_bits_of asid) of
     None \<Rightarrow> return ()
   | Some pool_ptr \<Rightarrow>  do
      pool \<leftarrow> get_asid_pool pool_ptr;
-     when (pool (ucast asid) = Some pd) $ do
+     when (pool (ucast asid) = Some pt) $ do
                 flush_space asid;
                 invalidate_asid_entry asid;
                 pool' \<leftarrow> return (pool (ucast asid := None));
@@ -360,22 +342,33 @@ delete_asid :: "asid \<Rightarrow> word32 \<Rightarrow> (unit,'z::state_ext) s_m
 od"
 
 text {* Switch to a particular address space in order to perform a flush
-operation. *}
+operation. Assumes pt is a level 1 table. *}
 definition
 set_vm_root_for_flush :: "word32 \<Rightarrow> asid \<Rightarrow> (bool,'z::state_ext) s_monad" where
-"set_vm_root_for_flush pd asid \<equiv> do
+"set_vm_root_for_flush pt asid \<equiv> do
     tcb \<leftarrow> gets cur_thread;
     thread_root_slot \<leftarrow> return (tcb, tcb_cnode_index 1);
     thread_root \<leftarrow> get_cap thread_root_slot;
-    not_is_pd \<leftarrow> (case thread_root of
-                    ArchObjectCap (PageDirectoryCap cur_pd (Some _)) \<Rightarrow> return (cur_pd \<noteq> pd)
+    not_is_pt \<leftarrow> (case thread_root of
+                    ArchObjectCap (PageTableCap _ cur_pt (Some _)) \<Rightarrow> return (cur_pt \<noteq> pt)
                   | _ \<Rightarrow> return True);
-    (if not_is_pd then do
-        arm_context_switch pd asid;
+    (if not_is_pt then do
+        arm_context_switch pt asid;
         return True
     od
     else return False)
 od"
+
+text {* Encoding of a device id in a word *}
+consts
+  device_id_from_word :: "machine_word \<Rightarrow> device_id"
+  word_from_device_id :: "device_id \<Rightarrow> machine_word"
+
+definition
+  invalidate_io_tlb_by_device :: "device_id \<Rightarrow> (unit, 'z::state_ext) s_monad"
+where
+  "invalidate_io_tlb_by_device dev \<equiv>
+    do_machine_op $ invalidateDeviceIOTLB (word_from_device_id dev)"
 
 definition
 do_flush :: "flush_type \<Rightarrow> vspace_ref \<Rightarrow> vspace_ref \<Rightarrow> paddr \<Rightarrow> unit machine_monad" where
@@ -394,83 +387,109 @@ do_flush :: "flush_type \<Rightarrow> vspace_ref \<Rightarrow> vspace_ref \<Righ
 
 text {* Flush mappings associated with a page table. *}
 definition
-flush_table :: "word32 \<Rightarrow> asid \<Rightarrow> vspace_ref \<Rightarrow> word32 \<Rightarrow> (unit,'z::state_ext) s_monad" where
-"flush_table pd asid vptr pt \<equiv> do
-    assert (vptr && mask (pageBitsForSize ARMSection) = 0);
-    root_switched \<leftarrow> set_vm_root_for_flush pd asid;
-    maybe_hw_asid \<leftarrow> load_hw_asid asid;
-    when (maybe_hw_asid \<noteq> None) $ do
-      hw_asid \<leftarrow> return (the maybe_hw_asid);
-      do_machine_op $ invalidateTLB_ASID hw_asid;
-      when root_switched $ do
-        tcb \<leftarrow> gets cur_thread;
-        set_vm_root tcb
+flush_table :: "word32 \<Rightarrow> mapping_root \<Rightarrow> vspace_ref \<Rightarrow> (unit,'z::state_ext) s_monad" where
+"flush_table pt m vptr \<equiv> 
+  case m of
+    MappedMem asid \<Rightarrow>
+    do
+      assert (vptr && mask (page_bits_for_size ARM_2M_Block) = 0);
+      root_switched \<leftarrow> set_vm_root_for_flush pt asid;
+      maybe_hw_asid \<leftarrow> load_hw_asid asid;
+      when (maybe_hw_asid \<noteq> None) $ do
+        hw_asid \<leftarrow> return (the maybe_hw_asid);
+        do_machine_op $ invalidateTLB_ASID hw_asid;
+        when root_switched $ do
+          tcb \<leftarrow> gets cur_thread;
+          set_vm_root tcb
+        od
       od
     od
-od"
+  | MappedIO device \<Rightarrow> invalidate_io_tlb_by_device device"
 
 text {* Flush mappings associated with a given page. *}
 definition
-flush_page :: "vmpage_size \<Rightarrow> word32 \<Rightarrow> asid \<Rightarrow> vspace_ref \<Rightarrow> (unit,'z::state_ext) s_monad" where
-"flush_page page_size pd asid vptr\<equiv> do
-    assert (vptr && mask pageBits = 0);
-    root_switched \<leftarrow> set_vm_root_for_flush pd asid;
-    maybe_hw_asid \<leftarrow> load_hw_asid asid;
-    when (maybe_hw_asid \<noteq> None) $ do
-      hw_asid \<leftarrow> return (the maybe_hw_asid);
-      do_machine_op $ invalidateTLB_VAASID (vptr || ucast hw_asid);
-      when root_switched $ do
-          tcb \<leftarrow> gets cur_thread;
-          set_vm_root tcb
+  flush_page :: "vmpage_size \<Rightarrow> word32 \<Rightarrow> mapping_root \<Rightarrow> vspace_ref \<Rightarrow> (unit,'z::state_ext) s_monad"
+where
+"flush_page page_size pt m vptr \<equiv>
+  case m of MappedMem asid \<Rightarrow>
+    do
+      assert (vptr && mask pageBits = 0);
+      root_switched \<leftarrow> set_vm_root_for_flush pt asid;
+      maybe_hw_asid \<leftarrow> load_hw_asid asid;
+      when (maybe_hw_asid \<noteq> None) $ do
+        hw_asid \<leftarrow> return (the maybe_hw_asid);
+        do_machine_op $ invalidateTLB_VAASID (vptr || ucast hw_asid);
+        when root_switched $ do
+            tcb \<leftarrow> gets cur_thread;
+            set_vm_root tcb
+        od
       od
-   od
-od"
+    od
+  | MappedIO device \<Rightarrow> invalidate_io_tlb_by_device device"
 
-text {* Return the optional page directory a page table is mapped in. *}
-definition
-page_table_mapped :: "asid \<Rightarrow> vspace_ref \<Rightarrow> obj_ref \<Rightarrow> (obj_ref option,'z::state_ext) s_monad" where
-"page_table_mapped asid vaddr pt \<equiv> doE
-    pd \<leftarrow> find_pd_for_asid asid;
-    pd_slot \<leftarrow> returnOk $ lookup_pd_slot pd vaddr;
-    pde \<leftarrow> liftE $ get_pde pd_slot;
-    case pde of
-      PageTablePDE addr _ _ \<Rightarrow> returnOk $
-             if addrFromPPtr pt = addr then Some pd else None
+text {* Return the optional previous-level page a page table is mapped in. *}
+fun
+  page_table_mapped :: "mapping_root \<Rightarrow> vspace_ref \<Rightarrow> pt_level \<Rightarrow> obj_ref \<Rightarrow> (obj_ref option,'z::state_ext) s_monad"
+where
+"page_table_mapped m vaddr PT_L1 pt = return None"
+|
+"page_table_mapped m vaddr l pt =
+(doE
+    pt1 \<leftarrow> find_root_pt m;
+    pt_slot \<leftarrow> lookup_pt_slot l vaddr pt1;
+    pte \<leftarrow> liftE $ get_pte pt_slot;
+    case pte of
+      TablePTE addr _ \<Rightarrow> returnOk $
+             if addrFromPPtr pt = ucast addr << pt_bits then Some pt1 else None
     | _ \<Rightarrow> returnOk None
-odE <catch> (K $ return None)"
+odE <catch> (K $ return None))"
+
+fun pred_level :: "pt_level \<Rightarrow> pt_level" where
+  "pred_level PT_L2 = PT_L1" |
+  "pred_level PT_L3 = PT_L2"
+
 
 text {* Unmap a page table from its page directory. *}
 definition
-unmap_page_table :: "asid \<Rightarrow> vspace_ref \<Rightarrow> word32 \<Rightarrow> (unit,'z::state_ext) s_monad" where
-"unmap_page_table asid vaddr pt \<equiv> do
-    pdOpt \<leftarrow> page_table_mapped asid vaddr pt;
-    case pdOpt of
+unmap_page_table :: "mapping_root \<Rightarrow> vspace_ref \<Rightarrow> pt_level \<Rightarrow> word32 \<Rightarrow> (unit,'z::state_ext) s_monad" where
+"unmap_page_table m vaddr l pt \<equiv> do
+    ptOpt \<leftarrow> page_table_mapped m vaddr l pt;
+    case ptOpt of
       None \<Rightarrow> return ()
-    | Some pd \<Rightarrow> do
-        pd_slot \<leftarrow> return $ lookup_pd_slot pd vaddr;
-        store_pde pd_slot InvalidPDE;
-        do_machine_op $ cleanByVA_PoU pd_slot (addrFromPPtr pd_slot);
-        flush_table pd asid vaddr pt
+    | Some pt \<Rightarrow> do
+        pt_slot \<leftarrow> return $ pte_slot (pred_level l) pt vaddr;
+        store_pte pt_slot InvalidPTE;
+        do_machine_op $ cleanByVA_PoU pt_slot (addrFromPPtr pt_slot);
+        flush_table pt m vaddr
     od
 od"
 
+text {* Size of memory region corresponding to a PTE *}
+fun
+  vmpage_size_of_pte :: "pte \<Rightarrow> vmpage_size"
+where
+  "vmpage_size_of_pte (PagePTE _ _ _) = ARM_4K_Page" |
+  "vmpage_size_of_pte (Block_2M_PTE _ _ _) = ARM_2M_Block" |
+  "vmpage_size_of_pte (Block_1G_PTE _ _ _) = ARM_1G_Block"
+
+text {* 32 bit physical address associated with a PTE. 0 if invalid. *}
+fun
+  addr_from_pte :: "pte \<Rightarrow> obj_ref"
+where
+  "addr_from_pte InvalidPTE = 0" |
+  "addr_from_pte (TablePTE ref _) = ucast ref << pt_bits" |
+  "addr_from_pte (Block_1G_PTE ref _ _) = ucast ref << 30" |
+  "addr_from_pte (Block_2M_PTE ref _ _) = ucast ref << 21" |
+  "addr_from_pte (PagePTE ref _ _) = ucast ref << pageBits"
+
 text {* Check that a given frame is mapped by a given mapping entry. *}
 definition
-check_mapping_pptr :: "obj_ref \<Rightarrow> vmpage_size \<Rightarrow> (obj_ref + obj_ref) \<Rightarrow> (bool,'z::state_ext) s_monad" where
-"check_mapping_pptr pptr pgsz tablePtr \<equiv> case tablePtr of
-   Inl ptePtr \<Rightarrow> do
-     pte \<leftarrow> get_pte ptePtr;
-     return $ case pte of
-       SmallPagePTE x _ _ \<Rightarrow> x = addrFromPPtr pptr \<and> pgsz = ARMSmallPage
-     | LargePagePTE x _ _ \<Rightarrow> x = addrFromPPtr pptr \<and> pgsz = ARMLargePage
-     | _ \<Rightarrow> False
-   od
- | Inr pdePtr \<Rightarrow> do
-     pde \<leftarrow> get_pde pdePtr;
-     return $ case pde of
-       SectionPDE x _ _ _ \<Rightarrow> x = addrFromPPtr pptr \<and> pgsz = ARMSection
-     | SuperSectionPDE x _ _ \<Rightarrow> x = addrFromPPtr pptr \<and> pgsz = ARMSuperSection
-     | _ \<Rightarrow> False
+  check_mapping_pptr :: "machine_word \<Rightarrow> vmpage_size \<Rightarrow> obj_ref \<Rightarrow> (bool,'z::state_ext) s_monad"
+where
+"check_mapping_pptr pptr pgsz pte_ref \<equiv> do
+     pte \<leftarrow> get_pte pte_ref;
+     return $ (is_block pte \<or> is_page pte) \<and> 
+              addrFromPPtr pptr = addr_from_pte pte \<and> pgsz = vmpage_size_of_pte pte
    od"
 
 text {* Raise an exception if a property does not hold. *}
@@ -478,89 +497,126 @@ definition
 throw_on_false :: "'e \<Rightarrow> (bool,'z::state_ext) s_monad \<Rightarrow> ('e + unit,'z::state_ext) s_monad" where
 "throw_on_false ex f \<equiv> doE v \<leftarrow> liftE f; unlessE v $ throwError ex odE"
 
+text {* Each page size can only occur on a specific page table level: *}
 definition
-  "last_byte_pte x \<equiv> let pte_bits = 2 in x + ((1 << pte_bits) - 1)"
-
-definition
-  "last_byte_pde x \<equiv> let pde_bits = 2 in x + ((1 << pde_bits) - 1)"
+  vmpage_size_to_level :: "vmpage_size \<Rightarrow> pt_level"
+where
+  "vmpage_size_to_level pgsz \<equiv> case pgsz of
+      ARM_4K_Page \<Rightarrow> PT_L3
+    | ARM_2M_Block \<Rightarrow> PT_L2
+    | ARM_1G_Block \<Rightarrow> PT_L1"
 
 text {* Unmap a mapped page if the given mapping details are still current. *}
 definition
-unmap_page :: "vmpage_size \<Rightarrow> asid \<Rightarrow> vspace_ref \<Rightarrow> obj_ref \<Rightarrow> (unit,'z::state_ext) s_monad" where
-"unmap_page pgsz asid vptr pptr \<equiv> doE
-    pd \<leftarrow> find_pd_for_asid asid;
-    (case pgsz of
-          ARMSmallPage \<Rightarrow> doE
-            p \<leftarrow> lookup_pt_slot pd vptr;
-            throw_on_false undefined $
-                check_mapping_pptr pptr pgsz (Inl p);
-            liftE $ do
-                store_pte p InvalidPTE;
-                do_machine_op $ cleanByVA_PoU p (addrFromPPtr p)
-            od
-          odE
-        | ARMLargePage \<Rightarrow> doE
-            p \<leftarrow> lookup_pt_slot pd vptr;
-            throw_on_false undefined $
-                check_mapping_pptr pptr pgsz (Inl p);
-            liftE $ do
-                assert $ p && mask 6 = 0;
-                slots \<leftarrow> return (map (\<lambda>x. x + p) [0, 4  .e.  60]);
-                mapM (swp store_pte InvalidPTE) slots;
-                do_machine_op $ cleanCacheRange_PoU (hd slots) (last_byte_pte (last slots))
-                                                    (addrFromPPtr (hd slots))
-            od
-          odE
-        | ARMSection \<Rightarrow> doE
-            p \<leftarrow> returnOk (lookup_pd_slot pd vptr);
-            throw_on_false undefined $
-                check_mapping_pptr pptr pgsz (Inr p);
-            liftE $ do
-                store_pde p InvalidPDE;
-                do_machine_op $ cleanByVA_PoU p (addrFromPPtr p)
-            od
-          odE
-        | ARMSuperSection \<Rightarrow> doE
-            p \<leftarrow> returnOk (lookup_pd_slot pd vptr);
-            throw_on_false undefined $
-                check_mapping_pptr pptr pgsz (Inr p);
-            liftE $ do
-                assert $ p && mask 6 = 0;
-                slots \<leftarrow> return (map (\<lambda>x. x + p) [0, 4  .e.  60]);
-                mapM (swp store_pde InvalidPDE) slots;
-                do_machine_op $ cleanCacheRange_PoU (hd slots) (last_byte_pde (last slots))
-                                                    (addrFromPPtr (hd slots))
-            od
-          odE);
-    liftE $ flush_page pgsz pd asid vptr
+unmap_page :: "vmpage_size \<Rightarrow> mapping_root \<Rightarrow> vspace_ref \<Rightarrow> obj_ref \<Rightarrow> (unit,'z::state_ext) s_monad" where
+"unmap_page pgsz m vptr pptr \<equiv> doE
+    pt \<leftarrow> find_root_pt m;
+    pte_ref \<leftarrow> lookup_pt_slot (vmpage_size_to_level pgsz) pt vptr;
+    throw_on_false undefined $ check_mapping_pptr pptr pgsz pte_ref;
+    liftE $ do
+      store_pte pte_ref InvalidPTE;
+      do_machine_op $ cleanByVA_PoU pte_ref (addrFromPPtr pte_ref);
+      flush_page pgsz pt m vptr
+    od
 odE <catch> (K $ return ())"
 
 
-text {* PageDirectory and PageTable capabilities cannot be copied until they
-have a virtual ASID and location assigned. This is because page directories
-cannot have multiple current virtual ASIDs and page tables cannot be shared
+
+text {* PageTable capabilities cannot be copied until they
+have a virtual ASID and location assigned. This is because page tables
+cannot have multiple current virtual ASIDs and cannot be shared
 between address spaces or virtual locations. *}
 definition
   arch_derive_cap :: "arch_cap \<Rightarrow> (arch_cap,'z::state_ext) se_monad"
 where
   "arch_derive_cap c \<equiv> case c of
-     PageTableCap _ (Some x) \<Rightarrow> returnOk c
-   | PageTableCap _ None \<Rightarrow> throwError IllegalOperation
-   | PageDirectoryCap _ (Some x) \<Rightarrow> returnOk c
-   | PageDirectoryCap _ None \<Rightarrow> throwError IllegalOperation
+     PageTableCap _ _ (Some x) \<Rightarrow> returnOk c
+   | PageTableCap _ _ None \<Rightarrow> throwError IllegalOperation
    | PageCap r R pgs x \<Rightarrow> returnOk (PageCap r R pgs None)
    | ASIDControlCap \<Rightarrow> returnOk c
-   | ASIDPoolCap _ _ \<Rightarrow> returnOk c"
+   | ASIDPoolCap _ _ \<Rightarrow> returnOk c
+   | IOSpaceCap _ \<Rightarrow> returnOk c
+   | VCPUCap _ \<Rightarrow> returnOk c"
 
-text {* No user-modifiable data is stored in ARM-specific capabilities. *}
+
+text {* Only IOSpaceCaps can be minted into new form. *}
 definition
-  arch_update_cap_data :: "data \<Rightarrow> arch_cap \<Rightarrow> cap"
+  arch_update_cap_data :: "data \<Rightarrow> arch_cap \<Rightarrow> arch_cap"
 where
-  "arch_update_cap_data data c \<equiv> ArchObjectCap c"
+  "arch_update_cap_data data c \<equiv> case c of
+     IOSpaceCap None \<Rightarrow> IOSpaceCap (Some (device_id_from_word data))
+   |  _ \<Rightarrow> c"
 
+text {* Unmap the page table associated with a device *}
+definition
+  unmap_device :: "device_id \<Rightarrow> (unit,'z::state_ext) s_monad"
+where
+  "unmap_device dev \<equiv> do
+    io_space \<leftarrow> gets (arm_io_space \<circ> arch_state);
+    io_space' \<leftarrow> return (io_space (dev := None));
+    modify (\<lambda>s. s\<lparr>arch_state := arch_state s \<lparr>arm_io_space := io_space'\<rparr>\<rparr>);
+    invalidate_io_tlb_by_device dev
+  od"
 
-text {* Actions that must be taken on finalisation of ARM-specific
-capabilities. *}
+text {* Unmap page table from device if provided PT is mapped there. *}
+definition
+  unmap_device_checked :: "device_id \<Rightarrow> obj_ref \<Rightarrow> (unit,'z::state_ext) s_monad"
+where
+  "unmap_device_checked dev pt \<equiv> do
+    opt_pt \<leftarrow> get_io_pt dev;
+    when (opt_pt = Some pt) $ unmap_device dev
+  od"
+
+text {* Map a page table to an empty device slot. *}
+definition
+  map_device :: "device_id \<Rightarrow> obj_ref \<Rightarrow> (unit,'z::state_ext) s_monad" where
+  "map_device dev pt_ref \<equiv> do
+    modify (arch_state_update (arm_io_space_update (\<lambda>io_space. io_space (dev \<mapsto> pt_ref))));
+    invalidate_io_tlb_by_device dev
+  od"
+
+text {* Invalidate appropriate TLB *}
+definition
+  "invalidate_tlb_by_mapping_root m \<equiv> case m of
+     MappedMem asid \<Rightarrow> invalidate_tlb_by_asid asid
+   | MappedIO dev \<Rightarrow> invalidate_io_tlb_by_device dev"
+
+text {* Dissociate a VCPU from a TCB *}
+definition
+  dissociate_vcpu :: "obj_ref \<Rightarrow> (unit,'z::state_ext) s_monad"
+where
+  "dissociate_vcpu vcpu \<equiv> do
+    (tcb_opt, r) \<leftarrow> get_vcpu vcpu;
+    case tcb_opt of
+      None \<Rightarrow> return ()
+    | Some tcb \<Rightarrow> do
+        thread_set (\<lambda>t. t \<lparr> tcb_vcpu := None \<rparr>) tcb;
+        set_vcpu vcpu (None, r)
+      od
+  od"
+
+text {* Dissociate a TCB from a VCPU *}
+definition
+  dissociate_tcb :: "obj_ref \<Rightarrow> (unit,'z::state_ext) s_monad"
+where
+  "dissociate_tcb tcb_ref \<equiv> do
+    vcpu_opt \<leftarrow> thread_get tcb_vcpu tcb_ref;
+    case vcpu_opt of
+      None \<Rightarrow> return ()
+    | Some vcpu \<Rightarrow> dissociate_vcpu vcpu
+  od"
+
+text {* Associate a VCPU with a TCB *}
+definition
+  associate :: "obj_ref \<Rightarrow> obj_ref \<Rightarrow> (unit,'z::state_ext) s_monad"
+where
+  "associate vcpu_ref tcb_ref \<equiv> do
+    (_,r) \<leftarrow> get_vcpu vcpu_ref;
+    set_vcpu vcpu_ref (Some tcb_ref, r);
+    thread_set (tcb_vcpu_update $ K $ Some vcpu_ref) tcb_ref
+  od"
+
+text {* Actions that must be taken on finalisation of ARM-specific capabilities. *}
 definition
   arch_finalise_cap :: "arch_cap \<Rightarrow> bool \<Rightarrow> (cap,'z::state_ext) s_monad"
 where
@@ -569,17 +625,27 @@ where
     delete_asid_pool b ptr;
     return NullCap
     od
-  | (PageDirectoryCap ptr (Some a), True) \<Rightarrow> do
-    delete_asid a ptr;
+  | (PageTableCap l ptr (Some (m, v)), True) \<Rightarrow> do
+    if l = PT_L1 then
+      (case m of
+        MappedMem asid \<Rightarrow> delete_asid asid ptr
+      | MappedIO dev \<Rightarrow> unmap_device_checked dev ptr)
+    else unmap_page_table m v l ptr;
     return NullCap
   od
-  | (PageTableCap ptr (Some (a, v)), True) \<Rightarrow> do
-    unmap_page_table a v ptr;
-    return NullCap
-  od
-  | (PageCap ptr _ s (Some (a, v)), _) \<Rightarrow> do
-     unmap_page s a v ptr;
+  | (PageCap ptr _ s (Some (m, v)), _) \<Rightarrow> do
+     unmap_page s m v ptr;
      return NullCap
+  od
+  | (VCPUCap vcpu_ref, True) \<Rightarrow> do
+     dissociate_vcpu vcpu_ref;
+     return NullCap
+  od
+  | (IOSpaceCap dev_opt, True) \<Rightarrow> do
+      case dev_opt of
+        None \<Rightarrow> return ()
+      | Some dev \<Rightarrow> unmap_device dev;
+      return NullCap
   od
   | _ \<Rightarrow> return NullCap"
 
@@ -589,8 +655,7 @@ fun
   arch_reset_mem_mapping :: "arch_cap \<Rightarrow> arch_cap"
 where
   "arch_reset_mem_mapping (PageCap p rts sz mp) = PageCap p rts sz None"
-| "arch_reset_mem_mapping (PageTableCap ptr mp) = PageTableCap ptr None"
-| "arch_reset_mem_mapping (PageDirectoryCap ptr ma) = PageDirectoryCap ptr None"
+| "arch_reset_mem_mapping (PageTableCap l ptr mp) = PageTableCap l ptr None"
 | "arch_reset_mem_mapping cap = cap"
 
 text {* Actions that must be taken to recycle ARM-specific capabilities. *}
@@ -599,37 +664,26 @@ definition
 where
   "arch_recycle_cap is_final cap \<equiv> case cap of
     PageCap p _ sz _ \<Rightarrow> do
-      do_machine_op $ clearMemory p (2 ^ (pageBitsForSize sz));
+      do_machine_op $ clearMemory p (2 ^ (page_bits_for_size sz));
       arch_finalise_cap cap is_final;
       return $ arch_reset_mem_mapping cap
     od
-  | PageTableCap ptr mp \<Rightarrow> do
-      pte_bits \<leftarrow> return 2;
+  | PageTableCap level ptr mp \<Rightarrow> do
+      pte_bits \<leftarrow> return 3;
       slots \<leftarrow> return [ptr, ptr + (1 << pte_bits) .e. ptr + (1 << pt_bits) - 1];
       mapM_x (swp store_pte InvalidPTE) slots;
-      do_machine_op $ cleanCacheRange_PoU ptr (ptr + (1 << pt_bits) - 1)
-                                          (addrFromPPtr ptr);
-      case mp of None \<Rightarrow> return ()
-       | Some (a, v) \<Rightarrow> do
-          pdOpt \<leftarrow> page_table_mapped a v ptr;
-          when (pdOpt \<noteq> None) $ invalidate_tlb_by_asid a
-          od;
-      arch_finalise_cap cap is_final;
-      return (if is_final then arch_reset_mem_mapping cap else cap)
-    od
-  | PageDirectoryCap ptr ma \<Rightarrow> do
-      pde_bits \<leftarrow> return 2;
-      indices \<leftarrow> return [0 .e. (kernel_base >> pageBitsForSize ARMSection) - 1];
-      offsets \<leftarrow> return (map (swp (op <<) pde_bits) indices);
-      slots \<leftarrow> return (map (\<lambda>x. x + ptr) offsets);
-      mapM_x (swp store_pde InvalidPDE) slots;
-      do_machine_op $ cleanCacheRange_PoU ptr (ptr + (1 << pd_bits) - 1)
-                                          (addrFromPPtr ptr);
-      case ma of None \<Rightarrow> return ()
-               | Some a \<Rightarrow> doE
-                            pd' \<leftarrow> find_pd_for_asid a;
-                            liftE $ when (pd' = ptr) $ invalidate_tlb_by_asid a
-                           odE <catch> K (return ());
+      do_machine_op $ cleanCacheRange_PoU ptr (ptr + (1 << pt_bits) - 1) (addrFromPPtr ptr);
+      case mp of 
+         None \<Rightarrow> return ()
+       | Some (m, v) \<Rightarrow>
+           if level = PT_L1 then doE
+             pt \<leftarrow> find_root_pt m;
+             whenE (pt = ptr) $ liftE $ invalidate_tlb_by_mapping_root m
+           odE <catch> K (return ())
+           else do
+             pt_opt \<leftarrow> page_table_mapped m v level ptr;
+             when (pt_opt \<noteq> None) $ invalidate_tlb_by_mapping_root m
+           od;
       arch_finalise_cap cap is_final;
       return (if is_final then arch_reset_mem_mapping cap else cap)
     od
@@ -644,13 +698,14 @@ where
           modify (\<lambda>s. s \<lparr> arch_state := (arch_state s) \<lparr> arm_asid_table := asid_table' \<rparr>\<rparr>)
       od;
       return cap
-    od"
+    od
+  | IOSpaceCap dev_opt \<Rightarrow> return cap
+  | VCPUCap vcpu_ref \<Rightarrow> return cap"
 
-text {* A thread's virtual address space capability must be to a page directory
-to be valid on the ARM architecture. *}
+text {* A thread's virtual address space capability must be to a level 1 page table. *}
 definition
   is_valid_vtable_root :: "cap \<Rightarrow> bool" where
-  "is_valid_vtable_root c \<equiv> \<exists>r a. c = ArchObjectCap (PageDirectoryCap r (Some a))"
+  "is_valid_vtable_root c \<equiv> \<exists>r a v. c = ArchObjectCap (PageTableCap PT_L1 r (Some (MappedMem a, v)))"
 
 text {* A thread's IPC buffer capability must be to a page that is capable of
 containing the IPC buffer without the end of the buffer spilling into another
@@ -717,9 +772,9 @@ attribs_from_word :: "word32 \<Rightarrow> vm_attributes" where
 
 text {* Update the mapping data saved in a page or page table capability. *}
 definition
-  update_map_data :: "arch_cap \<Rightarrow> (word32 \<times> word32) option \<Rightarrow> arch_cap" where
+  update_map_data :: "arch_cap \<Rightarrow> (mapping_root \<times> vspace_ref) option \<Rightarrow> arch_cap" where
   "update_map_data cap m \<equiv> case cap of PageCap p R sz _ \<Rightarrow> PageCap p R sz m
-                                     | PageTableCap p _ \<Rightarrow> PageTableCap p m"
+                                     | PageTableCap l p _ \<Rightarrow> PageTableCap l p m"
 
 text {* Get information about the frame of a given virtual address *}
 definition
